src/typechecker/FStar.TypeChecker.Normalize.fst
@@ -863,6 +863,20 @@ let is_forall_const cfg (phi : term) : option term =
 
     | _ -> None
 
+let is_extract_as_attr (attr: attribute) : option term =
+  let head, args = head_and_args attr in
+  match (Subst.compress head).n, args with
+  | Tm_fvar fv, [t, _] when Syntax.fv_eq_lid fv PC.extract_as_lid ->
+    (match (Subst.compress t).n with
+    | Tm_quoted(impl, _) -> Some impl
+    | _ -> None)
+  | _ -> None
+
+let has_extract_as_attr (g: Env.env) (lid: I.lid) : option term =
+  match Env.lookup_attrs_of_lid g lid with
+  | Some attrs -> find_map attrs is_extract_as_attr
+  | None -> None
+
 (* GM: Please consider this function private outside of this recursive
  * group, and call `normalize` instead. `normalize` will print timing
  * information when --debug NormTop is given, which makes it a
@@ -1498,7 +1512,20 @@ let rec norm : cfg -> env -> stack -> term -> term =
 (* NOTE: we do not need any environment here, since an fv does not
  * have any free indices. Hence, we use empty_env as environment when needed. *)
 and do_unfold_fv (cfg:Cfg.cfg) stack (t0:term) (qninfo : qninfo) (f:fv) : term =
-    match Env.lookup_definition_qninfo cfg.delta_level f.fv_name.v qninfo with
+    // Second, try to unfold to the definition itself.
+    let defn () = Env.lookup_definition_qninfo cfg.delta_level f.fv_name.v qninfo in
+    // First, try to unfold to the implementation specified in the extract_as attribute (when doing extraction)
+    let defn () =
+      if cfg.steps.for_extraction then
+        match qninfo with
+        | Some (Inr (se, None), _) when Env.visible_with cfg.delta_level se.sigquals ->
+          (match find_map se.sigattrs is_extract_as_attr with
+          | Some impl -> Some ([], impl)
+          | None -> defn ())
+        | _ -> defn ()
+      else
+        defn () in
+    match defn () with
        | None ->
          log_unfolding cfg (fun () ->
            BU.print2 " >> No definition found for %s (delta_level = %s)\n"
