src/parser/FStar.Parser.Const.fst
@@ -598,4 +598,5 @@ let tref_lid        = p2l ["FStar"; "Stubs"; "Tactics"; "Types"; "tref"]
 let document_lid = p2l ["FStar"; "Stubs"; "Pprint"; "document"]
 let issue_lid = p2l ["FStar"; "Issue"; "issue"]
 
+let extract_as_lid = p2l ["FStar"; "ExtractAs"; "extract_as"]
 let extract_as_impure_effect_lid = p2l ["FStar"; "Pervasives"; "extract_as_impure_effect"]
